iris_heap_lang/adequacy.v
@@ -25,18 +25,18 @@ with a non-constant step index function. We thus use the more general
 [wp_adequacy], and it hence would make sense to see if we can prove a version
 of [wp_adequacy] for a non-constant step version. *)
 Definition heap_adequacy Σ `{!heapGpreS Σ} s e σ φ :
-  (∀ `{!heapGS Σ, !HasLc Σ}, ⊢ inv_heap_inv -∗ WP e @ s; ⊤ {{ v, ⌜φ v⌝ }}) →
+  (∀ `{!heapGS Σ}, ⊢ inv_heap_inv -∗ WP e @ s; ⊤ {{ v, ⌜φ v⌝ }}) →
   adequate s e σ (λ v _, φ v).
 Proof.
   intros Hwp.
   apply adequate_alt; intros t2 σ2 [n [κs ?]]%erased_steps_nsteps.
-  eapply (wp_strong_adequacy_lc Σ _); [|done].
-  iIntros (Hinv HC).
+  eapply (wp_strong_adequacy Σ _); [|done].
+  iIntros (Hinv).
   iMod (gen_heap_init σ.(heap)) as (?) "[Hh _]".
   iMod (inv_heap_init loc (option val)) as (?) ">Hi".
   iMod (proph_map_init κs σ.(used_proph_id)) as (?) "Hp".
   iMod (mono_nat_own_alloc) as (γ) "[Hsteps _]".
-  iDestruct (Hwp (HeapGS _ _ _ _ _ _ _) with "Hi") as "Hwp".
+  iDestruct (Hwp (HeapGS _ _ _ _ _ _ _ _) with "Hi") as "Hwp".
   iModIntro.
   iExists (λ σ ns κs nt, (gen_heap_interp σ.(heap) ∗
                           proph_map_interp κs σ.(used_proph_id) ∗
